src/Decidable.v
@@ -1,0 +1,54 @@
+(** Typeclass for decidable propositions *)
+(** simplification of  fiat-crypto/src/Util/Decidable.v *)
+
+Require Import Coq.Arith.PeanoNat.
+Require Import Coq.Arith.Compare_dec.
+Require Import Coq.ZArith.BinInt.
+Require Import Coq.NArith.NArith.
+Require Import bbv.Word.
+Require Import bbv.NLib.
+
+Class Decidable (P : Prop) := dec : {P} + {~P}.
+Arguments dec _%type_scope {_}.
+
+Notation DecidableRel R := (forall x y, Decidable (R x y)).
+Notation DecidableEq T := (forall (x y: T), Decidable (x = y)).
+
+Global Instance dec_eq_nat : DecidableEq nat := Nat.eq_dec.
+Global Instance dec_le_nat : DecidableRel le := Compare_dec.le_dec.
+Global Instance dec_lt_nat : DecidableRel lt := Compare_dec.lt_dec.
+Global Instance dec_ge_nat : DecidableRel ge := Compare_dec.ge_dec.
+Global Instance dec_gt_nat : DecidableRel gt := Compare_dec.gt_dec.
+
+Global Instance dec_eq_Z : DecidableEq Z := Z.eq_dec.
+Global Instance dec_lt_Z : DecidableRel BinInt.Z.lt := ZArith_dec.Z_lt_dec.
+Global Instance dec_le_Z : DecidableRel BinInt.Z.le := ZArith_dec.Z_le_dec.
+Global Instance dec_gt_Z : DecidableRel BinInt.Z.gt := ZArith_dec.Z_gt_dec.
+Global Instance dec_ge_Z : DecidableRel BinInt.Z.ge := ZArith_dec.Z_ge_dec.
+
+Global Instance dec_eq_N : DecidableEq N := N.eq_dec.
+Global Instance dec_lt_N : DecidableRel N.lt := Nlt_dec.
+
+Global Instance decidable_eq_option {A} `{DecidableEq A}: DecidableEq (option A).
+  intros. unfold Decidable. destruct x; destruct y.
+  - destruct (DecidableEq0 a a0).
+    + subst. left. reflexivity.
+    + right. unfold not in *. intro E. inversion E. auto.
+  - right. intro. discriminate.
+  - right. intro. discriminate.
+  - left. reflexivity.
+Defined.
+
+Global Instance dec_and {A B} `{Decidable A, Decidable B} : Decidable (A /\ B).
+  unfold Decidable in *; destruct H; destruct H0; tauto.
+Defined.
+
+Global Instance dec_or {A B} `{Decidable A, Decidable B} : Decidable (A \/ B).
+  unfold Decidable in *; destruct H; destruct H0; tauto.
+Defined.
+
+Global Instance dec_not {A} `{Decidable A} : Decidable (~ A).
+  unfold Decidable in *. destruct H; tauto.
+Defined.
+
+Global Instance dec_eq_word : forall sz, DecidableEq (word sz) := weq.
