src/NameWithEq.v
@@ -1,0 +1,6 @@
+Require Export compiler.Decidable.
+
+Class NameWithEq := mkNameWithEq {
+  name: Set;
+  eq_name_dec: DecidableEq name
+}.
