src/PipelineTest.v
@@ -2,7 +2,7 @@ Require Import Coq.Lists.List.
 Import ListNotations.
 Require Import lib.LibTacticsMin.
 Require Import bbv.Word.
-Require Import riscv.util.Decidable.
+Require Import compiler.Decidable.
 Require Import compiler.Op.
 Require Import compiler.ExprImp.
 Require Import compiler.NameGen.
@@ -11,7 +11,7 @@ Require Import compiler.Pipeline.
 Require Import riscv.Riscv.
 Require Import compiler.MyOmega.
 Require Import riscv.util.Monads.
-Require Import riscv.util.NameWithEq.
+Require Import compiler.NameWithEq.
 Require Import riscv.RiscvBitWidths.
 
 Require Import riscv.RiscvBitWidths32.
